src/spec/TLS13.Wire.Spec.Reveal.ClientHello.Parseback.Low.fsti
@@ -2,8 +2,10 @@ module TLS13.Wire.Spec.Reveal.ClientHello.Parseback.Low
 
 module B = TLS13.Bytes
 module M = TLS13.Messages
+module T = TLS13.Types
 module Seq = FStar.Seq
 module LP = LowParse.Spec
+module WS = TLS13.Wire.Spec
 module GPV = TLS13.Wire.Generated.ProtocolVersion
 module GCS = TLS13.Wire.Generated.CipherSuite
 module GComp = TLS13.Wire.Generated.ClientHello_legacy_compression_methods
@@ -22,6 +24,15 @@ val mk_ext_list_some
 val mk_ext_list_none
   (key: B.bytes{B.length key == 32})
   : GCHEXT.clientHello_extensions
+
+val mk_ch_low_some
+  (ch: M.client_hello{B.length ch.M.random == 32 /\ B.length ch.M.key_share == 32})
+  (hostname: B.bytes{B.length hostname <= 255 /\ B.length hostname > 0})
+  : GCH.clientHello
+
+val mk_ch_low_none
+  (ch: M.client_hello{B.length ch.M.random == 32 /\ B.length ch.M.key_share == 32})
+  : GCH.clientHello
 
 val lemma_lp_ch_ext_ser_some
   (hostname: B.bytes{B.length hostname <= 255 /\ B.length hostname > 0})
@@ -43,7 +54,9 @@ val lemma_lp_ch_ext_ser_none
         (TLS13.Wire.Spec.Reveal.ClientHello.client_hello_common_extensions_bytes key)))
 
 val lemma_lp_ch_low_bytes_some
-  (ch: M.client_hello{B.length ch.M.random == 32 /\ B.length ch.M.key_share == 32})
+  (ch: M.client_hello{B.length ch.M.random == 32 /\ B.length ch.M.key_share == 32 /\
+                       ch.M.cipher_suites == [T.TLS_CHACHA20_POLY1305_SHA256] /\
+                       ch.M.signature_schemes == [T.RsaPssRsaeSha256]})
   (hostname: B.bytes{B.length hostname <= 255 /\ B.length hostname > 0 /\ ch.M.server_name == Some hostname})
   : Lemma
       (let low : GCH.clientHello =
@@ -54,10 +67,21 @@ val lemma_lp_ch_low_bytes_some
            GCH.legacy_compression_methods = B.of_list [0uy];
            GCH.extensions = mk_ext_list_some hostname ch.M.key_share } in
        Seq.equal (LP.serialize GCH.clientHello_serializer low)
-                 (TLS13.Wire.Spec.Reveal.ClientHello.client_hello_body_bytes ch.M.random hostname ch.M.key_share))
+                 (TLS13.Wire.Spec.Reveal.ClientHello.client_hello_body_bytes ch.M.random hostname ch.M.key_share) /\
+       Seq.equal (LP.serialize GCH.clientHello_serializer low)
+                 (TLS13.Wire.Spec.Reveal.ClientHello.client_hello_body_bytes
+                   ch.M.random
+                   (match ch.M.server_name with
+                    | Some h -> h
+                    | None -> B.empty)
+                   ch.M.key_share) /\
+       WS.synth_client_hello low == Some ch)
 
 val lemma_lp_ch_low_bytes_none
-  (ch: M.client_hello{B.length ch.M.random == 32 /\ B.length ch.M.key_share == 32})
+  (ch: M.client_hello{B.length ch.M.random == 32 /\ B.length ch.M.key_share == 32 /\
+                       ch.M.cipher_suites == [T.TLS_CHACHA20_POLY1305_SHA256] /\
+                       ch.M.signature_schemes == [T.RsaPssRsaeSha256] /\
+                       ch.M.server_name == None})
   : Lemma
       (let low : GCH.clientHello =
          { GCH.legacy_version = GPV.TLS_1p2;
@@ -67,4 +91,60 @@ val lemma_lp_ch_low_bytes_none
            GCH.legacy_compression_methods = B.of_list [0uy];
            GCH.extensions = mk_ext_list_none ch.M.key_share } in
        Seq.equal (LP.serialize GCH.clientHello_serializer low)
-                 (TLS13.Wire.Spec.Reveal.ClientHello.client_hello_body_bytes ch.M.random B.empty ch.M.key_share))
+                 (TLS13.Wire.Spec.Reveal.ClientHello.client_hello_body_bytes ch.M.random B.empty ch.M.key_share) /\
+       Seq.equal (LP.serialize GCH.clientHello_serializer low)
+                 (TLS13.Wire.Spec.Reveal.ClientHello.client_hello_body_bytes
+                   ch.M.random
+                   (match ch.M.server_name with
+                    | Some h -> h
+                    | None -> B.empty)
+                   ch.M.key_share) /\
+       WS.synth_client_hello low == Some ch)
+
+val lemma_lp_ch_low_body_some
+  (ch: M.client_hello{B.length ch.M.random == 32 /\ B.length ch.M.key_share == 32 /\
+                      ch.M.cipher_suites == [T.TLS_CHACHA20_POLY1305_SHA256] /\
+                      ch.M.signature_schemes == [T.RsaPssRsaeSha256]})
+  (hostname: B.bytes{B.length hostname <= 255 /\ B.length hostname > 0 /\ ch.M.server_name == Some hostname})
+  : Lemma
+      (let low = mk_ch_low_some ch hostname in
+       Seq.equal (LP.serialize GCH.clientHello_serializer low)
+                (TLS13.Wire.Spec.Reveal.ClientHello.client_hello_body_bytes
+                  ch.M.random
+                  (match ch.M.server_name with
+                   | Some h -> h
+                   | None -> B.empty)
+                  ch.M.key_share))
+
+val lemma_lp_ch_low_body_none
+  (ch: M.client_hello{B.length ch.M.random == 32 /\ B.length ch.M.key_share == 32 /\
+                      ch.M.cipher_suites == [T.TLS_CHACHA20_POLY1305_SHA256] /\
+                      ch.M.signature_schemes == [T.RsaPssRsaeSha256] /\
+                      ch.M.server_name == None})
+  : Lemma
+      (let low = mk_ch_low_none ch in
+       Seq.equal (LP.serialize GCH.clientHello_serializer low)
+                (TLS13.Wire.Spec.Reveal.ClientHello.client_hello_body_bytes
+                  ch.M.random
+                  (match ch.M.server_name with
+                   | Some h -> h
+                   | None -> B.empty)
+                  ch.M.key_share))
+
+val lemma_lp_ch_low_synth_some
+  (ch: M.client_hello{B.length ch.M.random == 32 /\ B.length ch.M.key_share == 32 /\
+                      ch.M.cipher_suites == [T.TLS_CHACHA20_POLY1305_SHA256] /\
+                      ch.M.signature_schemes == [T.RsaPssRsaeSha256]})
+  (hostname: B.bytes{B.length hostname <= 255 /\ B.length hostname > 0 /\ ch.M.server_name == Some hostname})
+  : Lemma
+      (let low = mk_ch_low_some ch hostname in
+       WS.synth_client_hello low == Some ch)
+
+val lemma_lp_ch_low_synth_none
+  (ch: M.client_hello{B.length ch.M.random == 32 /\ B.length ch.M.key_share == 32 /\
+                      ch.M.cipher_suites == [T.TLS_CHACHA20_POLY1305_SHA256] /\
+                      ch.M.signature_schemes == [T.RsaPssRsaeSha256] /\
+                      ch.M.server_name == None})
+  : Lemma
+      (let low = mk_ch_low_none ch in
+       WS.synth_client_hello low == Some ch)
